examples/alist.v
@@ -1,0 +1,5 @@
+From cryptis.examples.alist Require Import impl proofs.
+
+Module AList.
+Include proofs.Impure.
+End AList.
