examples/alist/impl.v
@@ -1,0 +1,48 @@
+From cryptis Require Import lib.
+From stdpp Require Import base gmap.
+From mathcomp Require Import ssreflect.
+From stdpp Require Import namespaces.
+From iris.algebra Require Import agree auth csum gset gmap excl frac.
+From iris.algebra Require Import max_prefix_list.
+From iris.heap_lang Require Import notation proofmode.
+From iris.heap_lang.lib Require Import lock ticket_lock.
+From cryptis Require Import term cryptis primitives tactics.
+
+Set Implicit Arguments.
+Unset Strict Implicit.
+Unset Printing Implicit Defensive.
+
+Module Pure.
+
+Definition empty : val := λ: <>, []%V.
+
+Definition find : val := λ: "kvs" "k",
+  let: "res" := find_list (λ: "kv", eq_term (Fst "kv") "k") "kvs" in
+  match: "res" with
+    SOME "res" => SOME (Snd "res")
+  | NONE => NONE
+  end.
+
+Definition insert : val := λ: "kvs" "k" "v",
+  ("k", "v") :: "kvs".
+
+Definition delete : val := λ: "kvs" "k",
+  filter_list (λ: "p", ~ eq_term "k" (Fst "p")) "kvs".
+
+End Pure.
+
+Module Impure.
+
+Definition new : val := λ: <>,
+  ref (Pure.empty #()).
+
+Definition find : val := λ: "l" "k",
+  Pure.find !"l" "k".
+
+Definition insert : val := λ: "l" "k" "v",
+  "l" <- Pure.insert !"l" "k" "v".
+
+Definition delete : val := λ: "l" "k",
+  "l" <- Pure.delete !"l" "k".
+
+End Impure.
