examples/store/proofs/client/connect.v
@@ -8,7 +8,7 @@ From iris.base_logic.lib Require Import invariants.
 From iris.heap_lang Require Import notation proofmode.
 From cryptis Require Import lib term gmeta nown.
 From cryptis Require Import cryptis primitives tactics role.
-From cryptis.examples Require Import conn rpc.
+From cryptis.examples Require Import conn rpc alist.
 From cryptis.examples.store Require Import impl.
 From cryptis.examples.store.proofs Require Import base db.
 
