examples/store/proofs/server/create.v
@@ -5,8 +5,8 @@ From iris.algebra Require Import agree auth csum gset gmap excl frac.
 From iris.algebra Require Import max_prefix_list.
 From iris.heap_lang Require Import notation proofmode.
 From cryptis Require Import lib term cryptis primitives tactics role.
-From cryptis.examples Require Import iso_dh conn rpc.
-From cryptis.examples.store Require Import impl alist.
+From cryptis.examples Require Import iso_dh conn rpc alist.
+From cryptis.examples.store Require Import impl.
 From cryptis.examples.store.proofs Require Import base db.
 
 Set Implicit Arguments.
@@ -42,13 +42,13 @@ wp_list_match => [t1 t2 ->| ?]; wp_pures; last first.
 { iApply ("post" $! None). iFrame.
   iDestruct "inv_ts" as "[fail|inv_ts]"; eauto. }
 rewrite /=. iDestruct "p_ts" as "(p_t1 & p_t2 & _)".
-wp_bind (SAList.find _ _). iApply (SAList.wp_find with "db") => //.
+wp_bind (AList.find _ _). iApply (AList.wp_find with "db") => //.
 iIntros "!> db". rewrite lookup_fmap.
 case db_t1: (db !! t1) => [t2'|]; wp_pures.
 { iApply ("post" $! None). by iFrame. }
 iMod (create_resp with "ready inv_ts") as "[ready inv_ts]".
-wp_bind (SAList.insert _ _ _).
-iApply (SAList.wp_insert with "db").
+wp_bind (AList.insert _ _ _).
+iApply (AList.wp_insert with "db").
 iIntros "!> db". rewrite -fmap_insert. wp_pures.
 wp_list. wp_pures. iApply ("post" $! (Some _)).
 iModIntro. rewrite /= public_TInt. iFrame. iSplit => //.
